Iris/Iris/ProofMode/ClassesMake.lean
@@ -13,27 +13,78 @@ public meta import Iris.ProofMode.SynthInstance
 namespace Iris.ProofMode
 open Iris.BI
 
+/-- Aliases for [Affine] and [Absorbing], but the instances are severely
+restricted. They only inspect the top-level symbol or check if the whole BI
+is affine. -/
+@[rocq_alias QuickAffine]
+class QuickAffine [BI PROP] (P : PROP) where
+  quick_affine : Affine P
+export QuickAffine (quick_affine)
+@[rocq_alias QuickAbsorbing]
+class QuickAbsorbing [BI PROP] (P : PROP) where
+  quick_absorbing : Absorbing P
+export QuickAbsorbing (quick_absorbing)
+
+/-- The class [MakeSep P Q PQ] is used to compute `PQ := P ∗ Q`. -/
+@[rocq_alias MakeSep, rocq_alias KnownLMakeSep, rocq_alias KnownRMakeSep]
+class MakeSep [BI PROP] (P Q : PROP) (PQ : outParam PROP) where
+  make_sep : P ∗ Q ⊣⊢ PQ
+export MakeSep (make_sep)
+
+/-- The class [MakeAnd P Q PQ] is used to compute `PQ := P ∧ Q`. -/
+@[rocq_alias MakeAnd, rocq_alias KnownLMakeAnd, rocq_alias KnownRMakeAnd]
+class MakeAnd [BI PROP] (P Q : PROP) (PQ : outParam PROP) where
+  make_and : P ∧ Q ⊣⊢ PQ
+export MakeAnd (make_and)
+
+/-- The class [MakeOr P Q PQ] is used to compute `PQ := P ∨ Q`. -/
+@[rocq_alias MakeOr, rocq_alias KnownLMakeOr, rocq_alias KnownRMakeOr]
+class MakeOr [BI PROP] (P Q : PROP) (PQ : outParam PROP) where
+  make_or : P ∨ Q ⊣⊢ PQ
+export MakeOr (make_or)
+
 /-- The class [MakeAffinely P Q] is used to compute `Q := <affine> P`. -/
+@[rocq_alias MakeAffinely, rocq_alias KnownMakeAffinely]
 class MakeAffinely [BI PROP] (P : PROP) (Q : outParam PROP) where
   make_affinely : <affine> P ⊣⊢ Q
 export MakeAffinely (make_affinely)
 
 /-- The class [MakeIntuitionistically P Q] is used to compute `Q := □ P`. -/
+@[rocq_alias MakeIntuitionistically, rocq_alias KnownMakeIntuitionistically]
 class MakeIntuitionistically [BI PROP] (P : PROP) (Q : outParam PROP) where
   make_intuitionistically : □ P ⊣⊢ Q
 export MakeIntuitionistically (make_intuitionistically)
 
 /-- The class [MakeAbsorbingly P Q] is used to compute `Q := <absorb> P`. -/
+@[rocq_alias MakeAbsorbingly, rocq_alias KnownMakeAbsorbingly]
 class MakeAbsorbingly [BI PROP] (P : PROP) (Q : outParam PROP) where
   make_absorbingly : <absorb> P ⊣⊢ Q
 export MakeAbsorbingly (make_absorbingly)
 
 /-- The class [MakePersistently P Q] is used to compute `Q := <pers> P`. -/
+@[rocq_alias MakePersistently, rocq_alias KnownMakePersistently]
 class MakePersistently [BI PROP] (P : PROP) (Q : outParam PROP) where
   make_persistently : <pers> P ⊣⊢ Q
 export MakePersistently (make_persistently)
 
 /-- The class [MakeLaterN n P Q] is used to compute `lP := ▷^n P`. -/
+@[rocq_alias MakeLaterN, rocq_alias KnownMakeLaterN]
 class MakeLaterN [BI PROP] (n : Nat) (P : PROP) (lP : outParam PROP) where
   make_laterN : ▷^[n] P ⊣⊢ lP
 export MakeLaterN (make_laterN)
+
+/-- The class [MakeExcept0 P Q] is used to compute `Q := ◇ P`. -/
+@[rocq_alias MakeExcept0, rocq_alias KnownMakeExcept0]
+class MakeExcept0 [BI PROP] (P : PROP) (Q : outParam PROP) where
+  make_except0 : ◇ P ⊣⊢ Q
+export MakeExcept0 (make_except0)
+
+/-- The class [MakeBUpd P Q] is used to compute `Q := |==> P`. -/
+class MakeBUpd [BI PROP] [BIUpdate PROP] (P : PROP) (Q : outParam PROP) where
+  make_bupd : (|==> P) ⊣⊢ Q
+export MakeBUpd (make_bupd)
+
+/-- The class [MakeFUpd E1 E2 P Q] is used to compute `Q := |={E1, E2}=> P`. -/
+class MakeFUpd [BI PROP] [BIFUpdate PROP] (E1 E2 : CoPset) (P : PROP) (Q : outParam PROP) where
+  make_fupd : (|={E1,E2}=> P) ⊣⊢ Q
+export MakeFUpd (make_fupd)
