Iris/Iris/ProofMode/Tactics.lean
@@ -9,6 +9,7 @@ public meta import Iris.ProofMode.Tactics.Clear
 public meta import Iris.ProofMode.Tactics.Exact
 public meta import Iris.ProofMode.Tactics.ExFalso
 public meta import Iris.ProofMode.Tactics.Exists
+public meta import Iris.ProofMode.Tactics.Frame
 public meta import Iris.ProofMode.Tactics.Have
 public meta import Iris.ProofMode.Tactics.Intro
 public meta import Iris.ProofMode.Tactics.LeftRight
