Iris/Iris/ProofMode/Tactics/Frame.lean
@@ -1,0 +1,117 @@
+/-
+Copyright (c) 2026 Michael Sammler. All rights reserved.
+Released under Apache 2.0 license as described in the file LICENSE.
+Authors: Michael Sammler
+-/
+module
+
+import Iris.BI
+import Iris.ProofMode.Classes
+public meta import Iris.ProofMode.Patterns.SelPattern
+public meta import Iris.ProofMode.Tactics.Basic
+
+namespace Iris.ProofMode
+
+public section
+open BI
+
+theorem frame [BI PROP] {p} {e e' P Q R : PROP}
+    [h1 : Frame p R P Q]
+    (h2 : e ⊣⊢ e' ∗ □?p R) :
+    (e' ⊢ Q) →
+    e ⊢ P := λ h =>
+  h2.1.trans <| sep_comm.1.trans <| (sep_mono_r h).trans h1.1
+
+theorem frame_pure [BI PROP] {e P Q : PROP} (φ : Prop)
+    [h1 : Frame true iprop(⌜φ⌝) P Q] (h : φ) :
+    (e ⊢ Q) →
+    e ⊢ P := fun hQ =>
+  have h_box : emp ⊢ □?true iprop(⌜φ⌝) := affinely_intro ((pure_intro h).trans persistent)
+  emp_sep.2.trans <| (sep_mono_l h_box).trans <| (sep_mono_r hQ).trans h1.1
+
+theorem frame_true_done [BI PROP] (P : PROP) : P ⊢ True :=
+  pure_intro .intro
+
+public meta section
+open Lean Elab Tactic Meta Qq Std
+
+private def iFrameSingle {prop : Q(Type u)} (bi : Q(BI $prop)) (e : Q($prop))
+    (hyps : Hyps bi e) (goal : Q($prop)) (sel : SelTarget) :
+    ProofModeM ((e' : Q($prop)) × (_ : Hyps bi e')
+      × (goal' : Q($prop)) × Q(($e' ⊢ $goal') → $e ⊢ $goal)) := do
+    match sel.target with
+    | .inl uniq =>
+      let ⟨e', hyps', _, out', p, _, hrem⟩ := hyps.remove false uniq
+      let goal' ← mkFreshExprMVarQ q($prop)
+      if let .some _ ← ProofModeM.trySynthInstanceQ q(Frame $p $out' $goal $goal') then
+        return ⟨e', hyps', goal', q(frame $hrem)⟩
+      if sel.explicit then
+         throwError "iframe: cannot frame {out'}"
+      else
+        return ⟨e, hyps, goal, q(λ x => x)⟩
+    | .inr fvar =>
+      let ty ← fvar.getType
+      if ! (← Meta.isProp ty) then
+        throwError "iframe: {← fvar.getUserName} is not a Prop"
+      have φ : Q(Prop) := ty
+      have t : Q($φ) := Expr.fvar fvar
+      let goal' ← mkFreshExprMVarQ q($prop)
+      if let .some _ ← ProofModeM.trySynthInstanceQ q(Frame true iprop(⌜$φ⌝) $goal $goal') then
+        return ⟨e, hyps, goal', q(frame_pure $φ $t)⟩
+      if sel.explicit then
+        throwError "iframe: cannot frame ⌜{φ}⌝"
+      else
+        return ⟨e, hyps, goal, q(λ x => x)⟩
+
+
+
+private structure FrameState {u} {prop : Q(Type u)} (bi : Q(BI $prop)) (origE origGoal : Q($prop)) where
+  (e : Q($prop)) (hyps : Hyps bi e) (goal : Q($prop))
+  pf : Q(($e ⊢ $goal) → ($origE ⊢ $origGoal))
+
+private def FrameState.frame {u prop bi origE origGoal} :
+    @FrameState u prop bi origE origGoal → SelTarget →
+    ProofModeM (FrameState bi origE origGoal) := λ st sel => do
+    let ⟨e', hyps', goal', pf⟩ ← iFrameSingle bi st.e st.hyps st.goal sel
+    return { e := e', hyps := hyps', goal := goal', pf := q(λ h => $st.pf ($pf h)) }
+
+def iFrame {prop : Q(Type u)} (bi : Q(BI $prop)) (e : Q($prop))
+    (hyps : Hyps bi e) (goal : Q($prop)) (sels : List SelTarget) :
+    ProofModeM ((e' : Q($prop)) × (_ : Hyps bi e')
+      × (goal' : Q($prop)) × (Q(($e' ⊢ $goal') → $e ⊢ $goal) ⊕ Q($e ⊢ $goal))) := do
+  let mut st : FrameState bi e goal := { e, hyps, goal, pf := q(fun h => h) }
+  for sel in sels do st ← st.frame sel
+
+  -- try closing the goal for emp or True
+  let pf' ← match st.goal with
+    | ~q(iprop(emp)) =>
+      have e := st.e
+      if let .some _ ← trySynthInstanceQ q(Affine $e) then
+        return some (q(affine (P := $e)) : Q($e ⊢ $(st.goal)))
+      else
+        return none
+    | ~q(iprop(True)) =>
+      have e := st.e
+      return some (q(frame_true_done $e) : Q($e ⊢ $(st.goal)))
+    | _ => return none
+  if let some pf' := pf' then
+    have pf' : Q($st.e ⊢ $(st.goal)) := pf'
+    return ⟨_, st.hyps, st.goal, .inr q($(st.pf) $pf')⟩
+  return ⟨_, st.hyps, st.goal, .inl st.pf⟩
+
+
+elab "iframe" pats:(colGt selPat)+ : tactic => do
+  let pats ← liftMacroM <| SelPat.parse pats
+
+  ProofModeM.runTactic λ mvar { bi, e, hyps, goal, .. } => do
+  let pats ← SelPat.resolve hyps pats
+
+  let ⟨_, hyps', goal', pf⟩ ← iFrame bi e hyps goal pats
+  match pf with
+  | .inl pf =>
+    let pf' ← addBIGoal hyps' goal'
+    mvar.assign q($pf $pf')
+  | .inr pf =>
+    mvar.assign q($pf)
+
+macro "iframe" : tactic => `(tactic | iframe ∗)
